library/init/lean/compiler/ir/livevars.lean
@@ -112,18 +112,16 @@ private def bindVar (x : VarId) : Collector :=
 private def bindParams (ps : Array Param) : Collector :=
 λ s, ps.foldl (λ s p, s.erase p.x) s
 
-local infix ` >> `:50 := Function.comp
-
 def collectExpr : Expr → Collector
 | (Expr.ctor _ ys)       := collectArgs ys
 | (Expr.reset _ x)       := collectVar x
-| (Expr.reuse x _ _ ys)  := collectVar x >> collectArgs ys
+| (Expr.reuse x _ _ ys)  := collectVar x ∘ collectArgs ys
 | (Expr.proj _ x)        := collectVar x
 | (Expr.uproj _ x)       := collectVar x
 | (Expr.sproj _ _ x)     := collectVar x
 | (Expr.fap _ ys)        := collectArgs ys
 | (Expr.pap _ ys)        := collectArgs ys
-| (Expr.ap x ys)         := collectVar x >> collectArgs ys
+| (Expr.ap x ys)         := collectVar x ∘ collectArgs ys
 | (Expr.box _ x)         := collectVar x
 | (Expr.unbox x)         := collectVar x
 | (Expr.lit v)           := skip
@@ -131,26 +129,26 @@ def collectExpr : Expr → Collector
 | (Expr.isTaggedPtr x)   := collectVar x
 
 partial def collectFnBody : FnBody → JPLiveVarMap → Collector
-| (FnBody.vdecl x _ v b)    m := collectExpr v >> collectFnBody b m >> bindVar x
+| (FnBody.vdecl x _ v b)    m := collectExpr v ∘ collectFnBody b m ∘ bindVar x
 | (FnBody.jdecl j ys v b)   m :=
-  let jLiveVars := (collectFnBody v m >> bindParams ys) {} in
+  let jLiveVars := (collectFnBody v m ∘ bindParams ys) {} in
   let m         := m.insert j jLiveVars in
   collectFnBody b m
-| (FnBody.set x _ y b)      m := collectVar x >> collectArg y >> collectFnBody b m
-| (FnBody.setTag x _ b)     m := collectVar x >> collectFnBody b m
-| (FnBody.uset x _ y b)     m := collectVar x >> collectVar y >> collectFnBody b m
-| (FnBody.sset x _ _ y _ b) m := collectVar x >> collectVar y >> collectFnBody b m
-| (FnBody.inc x _ _ b)      m := collectVar x >> collectFnBody b m
-| (FnBody.dec x _ _ b)      m := collectVar x >> collectFnBody b m
-| (FnBody.del x b)          m := collectVar x >> collectFnBody b m
+| (FnBody.set x _ y b)      m := collectVar x ∘ collectArg y ∘ collectFnBody b m
+| (FnBody.setTag x _ b)     m := collectVar x ∘ collectFnBody b m
+| (FnBody.uset x _ y b)     m := collectVar x ∘ collectVar y ∘ collectFnBody b m
+| (FnBody.sset x _ _ y _ b) m := collectVar x ∘ collectVar y ∘ collectFnBody b m
+| (FnBody.inc x _ _ b)      m := collectVar x ∘ collectFnBody b m
+| (FnBody.dec x _ _ b)      m := collectVar x ∘ collectFnBody b m
+| (FnBody.del x b)          m := collectVar x ∘ collectFnBody b m
 | (FnBody.mdata _ b)        m := collectFnBody b m
 | (FnBody.ret x)            m := collectArg x
-| (FnBody.case _ x alts)    m := collectVar x >> collectArray alts (λ alt, collectFnBody alt.body m)
+| (FnBody.case _ x alts)    m := collectVar x ∘ collectArray alts (λ alt, collectFnBody alt.body m)
 | (FnBody.unreachable)      m := skip
-| (FnBody.jmp j xs)         m := collectJP m j >> collectArgs xs
+| (FnBody.jmp j xs)         m := collectJP m j ∘ collectArgs xs
 
 def updateJPLiveVarMap (j : JoinPointId) (ys : Array Param) (v : FnBody) (m : JPLiveVarMap) : JPLiveVarMap :=
-let jLiveVars := (collectFnBody v m >> bindParams ys) {} in
+let jLiveVars := (collectFnBody v m ∘ bindParams ys) {} in
 m.insert j jLiveVars
 
 end LiveVars
